working on erasure to x86-sc, removed some stuff from dry machine

concurrency/x86_safe.v
@@ -33,6 +33,334 @@ Import dry_context SEM mySchedule DryMachine DryMachine.ThreadPool.
 Set Bullet Behavior "None".
 Set Bullet Behavior "Strict Subproofs".
 
+
+(** ** Erasure from FineConc to X86-SC*)
+Module X86Erasure.
+
+  Require Import ccc26x86.Asm ccc26x86.Asm_coop.
+  Import event_semantics.
+  (*TODO: Things here should be abstracted to support similar
+  erasures, e.g. for Power, but due to time constraints I am going to
+  do it right away for now*)
+  
+  (**  The erased memory is identical for
+       everything but permissions. *)
+  Local Notation "a # b" := (PMap.get b a) (at level 1).
+
+  Record erasedMem (m m': mem) :=
+    { perm_le:
+        forall b ofs k,
+          (Mem.mem_access m')#b ofs k = Some Freeable;
+      erased_contents:
+       (Mem.mem_contents m') = (Mem.mem_contents m);
+      erased_nb: Mem.nextblock m = Mem.nextblock m'
+    }.
+
+  Definition erased_val v1 v2 : Prop :=
+    match v1, v2 with
+    | Vundef, _ => True
+    | v1, v2 => v1 = v2
+    end.
+  
+  Inductive erased_val_list : seq.seq val -> seq.seq val -> Prop :=
+    erased_val_nil : erased_val_list [::] [::]
+  | erased_val_cons : forall (v v' : val) (vl vl' : seq.seq val),
+      erased_val v v' ->
+      erased_val_list vl vl' ->
+      erased_val_list (v :: vl) (v' :: vl').
+    
+  Definition erased_reg (r:PregEq.t) (rs rs' : regset) : Prop :=
+    erased_val (Pregmap.get r rs) (Pregmap.get r rs').
+  
+  Definition erased_regs rs rs' : Prop :=
+    forall r, erased_reg r rs rs'.
+
+  Definition erased_loader (l l' : load_frame) : Prop :=
+    l = l'.
+
+  Definition erasedCores c c' :=
+    match c, c' with
+    | State rs loader, State rs' loader' =>
+      erased_regs rs rs' /\ erased_loader loader loader'
+    | Asm_CallstateIn vf args tys retty, Asm_CallstateIn vf' args' tys' retty' =>
+      vf = vf' /\ erased_val_list args args' /\
+      tys = tys' /\ retty = retty'
+    | Asm_CallstateOut ef vals rs loader, Asm_CallstateOut ef' vals' rs' loader' =>
+      ef = ef' /\ erased_val_list vals vals'
+      /\ erased_regs rs rs' /\ erased_loader loader loader'
+    | _, _ => False
+    end.
+
+  Definition erasedCtl c c' : Prop :=
+    match c, c' with
+    | Kinit vf arg, Kinit vf' arg' =>
+      erased_val vf vf' /\ erased_val arg arg'
+    | Krun c, Krun c' =>
+      erasedCores c c'
+    | Kblocked c, Kblocked c' =>
+      erasedCores c c'
+    | Kresume c arg, Kresume c' arg' =>
+      erasedCores c c' /\ erased_val arg arg'
+    | _, _  => False
+    end.
+
+  Inductive erased_threadPool tp (tp' : ErasedMachine.ThreadPool.t) :=
+    | ErasedPool :
+        num_threads tp = ErasedMachine.ThreadPool.num_threads tp' ->
+        (forall i (cnti: containsThread tp i)
+           (cnti': ErasedMachine.ThreadPool.containsThread tp' i),
+            erasedCtl (getThreadC cnti)
+                      (ErasedMachine.ThreadPool.getThreadC cnti')) ->
+        erased_threadPool tp tp'.
+
+  Lemma erased_val_refl:
+    forall v, erased_val v v.
+  Proof.
+    destruct v; simpl; auto.
+  Qed.
+
+  Hint Immediate erased_val_refl : erased.
+  Hint Constructors erased_val_list : erased.
+  
+  Lemma erased_val_list_refl:
+    forall vs, erased_val_list vs vs.
+  Proof with eauto with erased.
+    induction vs; simpl...
+  Qed.
+
+  Lemma erased_regs_refl:
+    forall rs, erased_regs rs rs.
+  Proof with eauto with erased.
+    intros rs r;
+    unfold erased_reg...
+  Qed.
+
+  Lemma erased_loader_refl:
+    forall loader, erased_loader loader loader.
+  Proof.
+    unfold erased_loader; auto.
+  Qed.
+  
+  Hint Immediate erased_regs_refl erased_loader_refl
+       erased_val_list_refl : erased.
+
+  Lemma erasedCores_refl:
+    forall c, erasedCores c c.
+  Proof with eauto with erased.
+    destruct c; simpl;
+    repeat split...
+  Qed.
+
+  Hint Immediate erasedCores_refl: erased.
+  
+  Lemma erasedCtl_refl:
+    forall c, erasedCtl c c.
+  Proof with eauto with erased.
+    destruct c; simpl...
+  Qed.
+  
+  Lemma erased_updLockSet:
+    forall tp tp' addr addr' rmap rmap',
+      erased_threadPool tp tp' ->
+      erased_threadPool (updLockSet tp addr rmap)
+                         (ErasedMachine.ThreadPool.updLockSet tp' addr' rmap').
+  Proof.
+    intros.
+    inversion H.
+    constructor; auto.
+  Qed.
+  
+  Lemma erased_updThread:
+    forall tp tp' i (cnti: containsThread tp i)
+      (cnti': ErasedMachine.ThreadPool.containsThread tp' i) c c' pmap pmap',
+      erased_threadPool tp tp' ->
+      erasedCtl c c' ->
+      erased_threadPool (updThread cnti c pmap)
+                        (ErasedMachine.ThreadPool.updThread cnti' c' pmap').
+  Proof.
+    intros.
+    inversion H.
+    constructor; auto.
+    intros.
+    destruct (i0 == i) eqn:Heq; move/eqP:Heq=>Heq.
+    subst. rewrite gssThreadCode.
+    rewrite ErasedMachine.ThreadPool.gssThreadCode; auto.
+    rewrite gsoThreadCode; auto.
+    rewrite ErasedMachine.ThreadPool.gsoThreadCode; auto.
+  Qed.
+
+  Lemma erased_addThread:
+    forall tp tp' i (cnti: containsThread tp i)
+      (cnti': ErasedMachine.ThreadPool.containsThread tp' i) v arg v' arg' pmap pmap',
+      erased_threadPool tp tp' ->
+      erased_val v v' ->
+      erased_val arg arg' ->
+      erased_threadPool (addThread tp v arg pmap)
+                        (ErasedMachine.ThreadPool.addThread tp' v arg pmap').
+  Proof with eauto with erased.
+    intros.
+    inversion H.
+    constructor.
+    unfold addThread, ErasedMachine.ThreadPool.addThread; simpl. rewrite H2; auto.
+    intros.
+    assert (cnti00 := cntAdd' _ _ _  cnti0).
+    assert (cnti0'0 := ErasedMachine.ThreadPool.cntAdd' _ _ _  cnti'0).
+    destruct cnti00 as [[cnti00 ?] | Heq];
+      destruct cnti0'0 as [[cnti0'0 ?] | ?].
+    - erewrite gsoAddCode with (cntj := cnti00) by eauto.
+      erewrite ErasedMachine.ThreadPool.gsoAddCode with (cntj := cnti0'0) by eauto.
+      eauto.
+    - exfalso; subst; apply H4.
+      destruct (num_threads tp), (ErasedMachine.ThreadPool.num_threads tp');
+        simpl; inversion H2; auto.
+    - exfalso; subst; apply H4.
+      destruct (num_threads tp), (ErasedMachine.ThreadPool.num_threads tp');
+        simpl; inversion H2; auto.
+    - subst. erewrite gssAddCode by eauto.
+      erewrite ErasedMachine.ThreadPool.gssAddCode; eauto.
+      simpl...
+  Qed.
+  
+  Lemma erased_remLockSet:
+    forall tp tp' addr addr',
+      erased_threadPool tp tp' ->
+      erased_threadPool (remLockSet tp addr)
+                         (ErasedMachine.ThreadPool.remLockSet tp' addr').
+  Proof.
+    intros.
+    inversion H.
+    constructor; auto.
+  Qed.
+
+  Lemma mem_load_erased:
+    forall chunk m m' b ofs pmap v
+      (Hlt: permMapLt pmap (getMaxPerm m))
+      (Hload: Mem.load chunk (restrPermMap Hlt) b ofs = Some v)
+      (Herased: erasedMem m m'),
+      Mem.load chunk m' b ofs = Some v.
+  Proof.
+    intros.
+    inversion Herased.
+    assert (Hreadable := Mem.load_valid_access _ _ _ _ _ Hload).
+    destruct Hreadable.
+    assert (Hreadable': Mem.valid_access m' chunk b ofs Readable).
+    { split; auto.
+      intros ? ?.
+      unfold Mem.perm.
+      rewrite perm_le0.
+      simpl; constructor.
+    }
+    Transparent Mem.load.
+    unfold Mem.load in *.
+    destruct (Mem.valid_access_dec m' chunk b ofs Readable);
+      try by exfalso.
+    destruct (Mem.valid_access_dec (restrPermMap Hlt) chunk b ofs Readable);
+      try by discriminate.
+    simpl in *.
+    rewrite erased_contents0; auto.
+    Opaque Mem.load.
+  Qed.
+
+  Lemma mem_store_erased:
+    forall chunk m m' b ofs pmap v m2
+      (Hv: v <> Vundef)
+      (Hlt: permMapLt pmap (getMaxPerm m))
+      (Hstore: Mem.store chunk (restrPermMap Hlt) b ofs v = Some m2)
+      (Herased: erasedMem m m'),
+    exists m2', Mem.store chunk m' b ofs v = Some m2'
+           /\ erasedMem m2 m2'.
+  Proof.
+    intros.
+    destruct Herased.
+    assert (Haccess := Mem.store_valid_access_3 _ _ _ _ _ _ Hstore).
+    destruct Haccess.
+    assert (Haccess' : Mem.valid_access m' chunk b ofs Writable).
+    { split; auto.
+      intros ? ?.
+      unfold Mem.perm.
+      rewrite perm_le0.
+      simpl; constructor.
+    }
+    Transparent Mem.store.
+    unfold Mem.store in *.
+    destruct (Mem.valid_access_dec m' chunk b ofs Writable); try by exfalso.
+    destruct (Mem.valid_access_dec (restrPermMap Hlt) chunk b ofs Writable);
+      try by discriminate. simpl in Hstore.
+    inv Hstore.
+    eexists; split; eauto.
+    constructor; simpl; auto.
+    rewrite <- erased_contents0.
+      reflexivity.
+    Opaque Mem.store.
+  Qed.
+  
+  Hint Resolve erased_updLockSet erased_updThread
+       erased_addThread erased_remLockSet mem_store_erased: erased.
+
+  Lemma at_external_erase:
+    forall c c' (Herase: erasedCores c c'),
+      match at_external Sem c, at_external Sem c' with
+      | Some (ef, sig, vs), Some (ef', sig', vs') =>
+        ef = ef' /\ sig = sig' /\ erased_val_list vs vs'
+      | None, None => True
+      | _, _ => False
+      end.
+  Admitted.
+
+  (** Simulation of synchronization steps between erased states*)
+
+    Lemma syncStep_erase:
+      forall ge tp1 tp1' m1 m1' tp2 m2 i ev
+        (HerasePool: erased_threadPool tp1 tp1')
+        (cnti: containsThread tp1 i)
+        (cnti': ErasedMachine.ThreadPool.containsThread tp1' i)
+        (HerasedMem: erasedMem m1 m1')
+        (Hcomp1: mem_compatible tp1 m1)
+        (Hcomp1': ErasedMachine.mem_compatible tp1' m1')
+        (Hstep: syncStep ge cnti Hcomp1 tp2 m2 ev),
+      exists tp2' m2',
+        ErasedMachine.syncStep ge cnti' Hcomp1' tp2' m2' ev /\
+        erased_threadPool tp2 tp2' /\ erasedMem m2 m2'.
+    Proof with eauto with erased.
+      intros.
+      inversion HerasePool as [Hnum Hthreads].
+      specialize (Hthreads _ cnti cnti').      
+      inversion Hstep; subst;
+      match goal with
+      | [H: erasedCtl ?Expr1 ?Expr2, H1: ?Expr1 = _ |- _] =>
+        rewrite H1 in H; simpl in H;
+        destruct Expr2 eqn:?
+      end; try (by exfalso);
+      try match goal with
+          | [H: Mem.load _ _ _ _ = Some _ |- _] =>
+            eapply mem_load_erased in H; eauto
+          end;
+      try match goal with
+          | [H: Mem.store _ _ _ _ _ = Some _ |- _] =>
+            eapply mem_store_erased in H; eauto;
+            destruct Hstore as [m2' [Hstore HerasedMem']]
+          end;
+      try match goal with
+          | [|- _ <> Vundef] => intro Hcontra; discriminate
+          end;
+      match goal with
+      | [H: at_external _ _ = _, H1: erasedCores _ _ |- _] =>
+        pose proof (at_external_erase _ _ H1);
+          match goal with
+          | [H2: match at_external _ _ with _ => _ end |- _] =>
+            rewrite H in H2;
+              match goal with
+              | [H3: match at_external ?E1 ?E2 with _ => _ end |- _] =>
+                destruct (at_external E1 E2) as [[[? ?] ?]|]; try by exfalso
+              end
+          end
+      end;
+      repeat match goal with
+             | [H: _ /\ _ |- _] => destruct H
+             end; subst.
+     Admitted.
+End X86Erasure.
+
 (** ** Safety for X86-SC semantics *)
 Module X86Safe.
   Import Asm Asm_coop event_semantics FineConcSafe Events.
